concurrency/node-replication/Interface.i.dfy
@@ -1,0 +1,107 @@
+include "Interface.s.dfy"
+include "Init.i.dfy"
+include "InfiniteLog_Refines_NRSimple.i.dfy"
+include "Linearize.i.dfy"
+
+module FilledInInterface(nifc: NRIfc)
+  refines Interface(
+    nifc,
+    InfiniteLogSSM(nifc),
+    NRSimple(nifc),
+    InfiniteLog_Refines_NRSimple(nifc)
+    //NRSimple_Refines_NRSingle(nifc) // XXX module system bug?
+  )
+{
+  import Impl = NRImpl(nifc)
+  import Init = Init(nifc)
+  import ILT = InfiniteLogTokens(nifc)
+  import IL = InfiniteLogSSM(nifc)
+  import opened LinearSequence_i`T
+
+  type GlobalState = Impl.NR
+  type NodeState = Impl.Node
+  type ThreadState = Impl.ThreadOwnedContext
+  type NodeInitToken = Init.NodeCreationToken
+
+  predicate WFGlobalState(gs: GlobalState) {
+    gs.WF()
+  }
+
+  predicate WFNodeInitToken(nit: NodeInitToken, gs: GlobalState) {
+    nit.WF(gs)
+  }
+
+  predicate WFNode(node: NodeState, gs: GlobalState) {
+    node.WF(gs)
+  }
+
+  predicate WFThread(t: ThreadState, node: NodeState, gs: GlobalState) {
+    t.WF(node, gs)
+  }
+
+  method init(glinear in_token: T.Token)
+  returns (linear gs: GlobalState, linear nodeCreationTokens: lseq<NodeInitToken>)
+  //requires in_token.loc == TicketStubSingletonLoc.loc()
+  //requires in_token.val == ssm.Init()
+  ensures WFGlobalState(gs)
+  ensures forall i | 0 <= i < |lseqs_raw(nodeCreationTokens)| ::
+      lseq_has(nodeCreationTokens)[i]
+        && WFNodeInitToken(read(lseqs_raw(nodeCreationTokens)[i]), gs)
+  {
+    gs, nodeCreationTokens := Init.initNR(in_token);
+    forall i | 0 <= i < |lseqs_raw(nodeCreationTokens)|
+        ensures lseq_has(nodeCreationTokens)[i]
+          && WFNodeInitToken(read(lseqs_raw(nodeCreationTokens)[i]), gs)
+    {
+      assert read(lseqs_raw(nodeCreationTokens)[i]) == nodeCreationTokens[i];
+      assert nodeCreationTokens[i].WF(gs);
+      assert read(lseqs_raw(nodeCreationTokens)[i]).WF(gs);
+    }
+  }
+
+  method initNode(shared gs: GlobalState, linear nit: NodeInitToken)
+  returns (linear node: NodeState, linear threads: lseq<ThreadState>)
+  //requires WFGlobalState(gs)
+  //requires WFNodeInitToken(nit, gs)
+  ensures WFGlobalState(gs)
+  ensures forall i | 0 <= i < |lseqs_raw(threads)| ::
+      lseq_has(threads)[i] && WFThread(read(lseqs_raw(threads)[i]), node, gs)
+  {
+    node, threads := Init.initNode(gs, nit);
+    forall i | 0 <= i < |lseqs_raw(threads)|
+    ensures lseq_has(threads)[i] && WFThread(read(lseqs_raw(threads)[i]), node, gs)
+    {
+      assert threads[i].WF(node, gs);
+    }
+  }
+
+  method do_operation(shared gs: GlobalState, shared node: NodeState,
+        linear inout t: ThreadState,
+        ghost rid: nat, input: nrifc.Input, glinear ticket: T.Token)
+  returns (output: nrifc.Output, glinear stub: T.Token)
+  decreases *
+  /*requires WFGlobalState(gs)
+  requires WFNode(node, gs)
+  requires WFThread(old_t, node, gs)
+  requires ticket.loc == TicketStubSingletonLoc.loc()
+  requires ticket.val == ssm.Ticket(rid, input)*/
+  ensures WFThread(t, node, gs)
+  ensures stub.loc == TicketStubSingletonLoc.loc()
+  ensures ssm.IsStub(rid, output, stub.val)
+  {
+    match input {
+      case ROp(rop) => {
+        glinear var folded_stub;
+        glinear var folded_ticket := ILT.Readonly_fold(ILT.Readonly(rid, IL.ReadonlyInit(rop)), ticket);
+        output, folded_stub, t := Impl.do_read(gs, node, rop, t, folded_ticket);
+        stub := ILT.Readonly_unfold(folded_stub);
+      }
+      case UOp(uop) => {
+        glinear var folded_stub;
+        glinear var folded_ticket := ILT.Update_fold(ILT.Update(rid, IL.UpdateInit(uop)), ticket);
+        output, folded_stub, t := Impl.do_update(gs, node, uop, folded_ticket, t);
+        stub := ILT.Update_unfold(folded_stub);
+      }
+    }
+  }
+}
