concurrency/node-replication/Interface.s.dfy
@@ -1,0 +1,65 @@
+include "NRSpec.s.dfy"
+include "Linearize.s.dfy"
+include "../framework/AsyncSSM.s.dfy"
+include "../framework/StateMachines.s.dfy"
+include "../../lib/Lang/LinearSequence.s.dfy"
+
+abstract module Interface(
+  nrifc: NRIfc,
+  ssm: TicketStubSSM(nrifc),
+  X: StateMachine(AsyncIfc(nrifc)),
+  refinement: Refinement(
+      AsyncIfc(nrifc),
+      TicketStubStateMachine(nrifc, ssm),
+      X)
+  //refinement2: Linearizer(nrifc, X)
+)
+{
+  import TicketStubSingletonLoc
+  import PCM = TicketStubPCM(nrifc, ssm)
+  import T = Tokens(PCM)
+  import opened GhostLoc
+  import opened LinearSequence_s
+  import opened LinearMaybe
+
+  type GlobalState
+  type NodeState
+  type ThreadState
+  type NodeInitToken
+
+  predicate WFGlobalState(gs: GlobalState)
+  predicate WFNodeInitToken(nit: NodeInitToken, gs: GlobalState)
+  predicate WFNode(node: NodeState, gs: GlobalState)
+  predicate WFThread(t: ThreadState, node: NodeState, gs: GlobalState)
+
+  method init(glinear in_token: T.Token)
+  returns (linear gs: GlobalState, linear nodeCreationTokens: lseq<NodeInitToken>)
+  requires in_token.loc == TicketStubSingletonLoc.loc()
+  requires in_token.val == ssm.Init()
+  ensures WFGlobalState(gs)
+  ensures forall i | 0 <= i < |lseqs_raw(nodeCreationTokens)| ::
+      lseq_has(nodeCreationTokens)[i]
+        && WFNodeInitToken(read(lseqs_raw(nodeCreationTokens)[i]), gs)
+
+  method initNode(shared gs: GlobalState, linear nit: NodeInitToken)
+  returns (linear node: NodeState, linear threads: lseq<ThreadState>)
+  requires WFGlobalState(gs)
+  requires WFNodeInitToken(nit, gs)
+  ensures WFGlobalState(gs)
+  ensures forall i | 0 <= i < |lseqs_raw(threads)| ::
+      lseq_has(threads)[i] && WFThread(read(lseqs_raw(threads)[i]), node, gs)
+
+  method do_operation(shared gs: GlobalState, shared node: NodeState,
+        linear inout t: ThreadState,
+        ghost rid: nat, input: nrifc.Input, glinear ticket: T.Token)
+  returns (output: nrifc.Output, glinear stub: T.Token)
+  decreases *
+  requires WFGlobalState(gs)
+  requires WFNode(node, gs)
+  requires WFThread(old_t, node, gs)
+  requires ticket.loc == TicketStubSingletonLoc.loc()
+  requires ticket.val == ssm.Ticket(rid, input)
+  ensures WFThread(t, node, gs)
+  ensures stub.loc == TicketStubSingletonLoc.loc()
+  ensures ssm.IsStub(rid, output, stub.val)
+}
