concurrency/node-replication/Linearize.s.dfy
@@ -1,0 +1,41 @@
+include "../framework/StateMachines.s.dfy"
+include "NRSpec.s.dfy"
+
+module Behavior(ifc: Ifc, sm: StateMachine(ifc)) {
+  datatype Behavior =
+    | Stepped(s: sm.Variables, op: sm.ifc.Op, tail: Behavior)
+    | Inited(s: sm.Variables)
+  {
+    predicate WF() {
+      match this {
+        case Stepped(s', op, tail) =>
+          && tail.WF()
+          && sm.Next(tail.s, s', op)
+        case Inited(s) =>
+          && sm.Init(s)
+      }
+    }
+  }
+}
+
+abstract module Linearizer(nrifc: NRIfc, simple: StateMachine(AsyncIfc(nrifc))) {
+  import one = AsyncStateMachine(nrifc, NROne(nrifc))
+
+  import SimpleB = Behavior(AsyncIfc(nrifc), simple)
+  import OneB = Behavior(AsyncIfc(nrifc), AsyncStateMachine(nrifc, NROne(nrifc)))
+
+  predicate equiv(a: SimpleB.Behavior, b: OneB.Behavior)
+  decreases a, b
+  {
+    || (a.Inited? && b.Inited?)
+    || (a.Stepped? && a.op.InternalOp? && equiv(a.tail, b))
+    || (b.Stepped? && b.op.InternalOp? && equiv(a, b.tail))
+    || (a.Stepped? && b.Stepped? && a.op == b.op && equiv(a.tail, b.tail))
+  }
+
+  lemma ExistsEquivBehavior(a: SimpleB.Behavior)
+  returns (b: OneB.Behavior)
+  requires a.WF()
+  ensures b.WF()
+  ensures equiv(a, b)
+}
